rocq/theories/TypeSystem/EnvRuntimeCapturedSafety.v
@@ -159,8 +159,7 @@ Lemma store_safe_synthetic_direct_call_ready_exact_body_call_route_scoped_packag
     component_body_synthetic_direct_call_ready_summary_at_check_in_provider env ->
     store_safe_synthetic_direct_call_ready_exact_body_call_route_scoped_package_statement
       (fun env0 fdef =>
-        exists bounds,
-          env0 = global_env_with_local_bounds env bounds /\
+        global_env_local_bounds_family env env0 /\
           In fdef (env_fns env) /\
           check_fn_root_shadow_no_capture_direct_call_component_store_safe_summary
             env fdef = true).
@@ -168,8 +167,9 @@ Proof.
   intros env Hunique Hsummary_provider.
   eapply store_safe_synthetic_direct_call_ready_exact_body_call_route_scoped_package_of_route_summary_at_provider.
   - intros env0 fname fdef fcall used used' fname_body args_body
-      synthetic_body (bounds & -> & Hin & Hcomponent_check) _Hin _Hname
+      synthetic_body (Hfamily & Hin & Hcomponent_check) _Hin _Hname
       Hrename Htarget.
+    destruct Hfamily as (bounds & ->).
     destruct (direct_call_target_expr_alpha_rename_fn_def_inv
                 used fdef fcall used' fname_body args_body synthetic_body
                 Hrename Htarget) as (args0 & Htarget_original).
@@ -177,7 +177,8 @@ Proof.
       as Hbounds.
     rewrite Hbounds.
     eapply Hsummary_provider; eassumption.
-  - intros env0 fdef (bounds & -> & _Hin & Hcomponent_check).
+  - intros env0 fdef (Hfamily & _Hin & Hcomponent_check).
+    destruct Hfamily as (bounds & ->).
     eapply callee_body_root_shadow_no_capture_direct_call_component_store_safe_summary_global_env_with_local_bounds.
     + exact Hunique.
     + eapply check_fn_root_shadow_no_capture_direct_call_component_store_safe_summary_sound.
